theories/examples/allocator.v
@@ -1,0 +1,121 @@
+From iris.base_logic Require Import invariants.
+From iris_ni.logrel Require Import types interp.
+From iris_ni.program_logic Require Import dwp heap_lang_lifting.
+From iris.proofmode Require Import tactics.
+From iris_ni.proofmode Require Import dwp_tactics.
+From iris.heap_lang Require Import lang array proofmode.
+From iris.algebra Require Import excl.
+
+From iris_ni.examples Require Import lock.
+
+Definition allocator_alloc : val :=
+  λ: "arr" "i" "sz" "v",
+  let: "pos" := !"i" in
+  if: ("sz" ≤ "pos")
+  then NONE
+  else "i" <- "pos" + #1;;
+       let: "c" := "arr" + "pos" in
+       "c" <- "v";;
+       SOME "c".
+
+Definition new_allocator : val :=
+  λ: "z",
+  let: "arr" := AllocN "z" NONE in
+  let: "i" := ref #0 in
+  let: "lk" := newlock #() in
+  (λ: "v", acquire "lk";;
+           let: "c" := allocator_alloc "arr" "i" "z" "v" in
+           release "lk";; "c").
+
+
+Section proof.
+  Context `{!heapDG Σ, !lockG Σ}.
+
+  Definition aN := nroot.@"allocator".
+
+  Definition allocator_inv l1 l2 i1 i2 sz : iProp Σ :=
+    (∃ i : Z, ⌜0 ≤ i ≤ sz⌝ ∗
+               (l1 +ₗ i) ↦ₗ∗ replicate (Z.to_nat (sz-i)) NONEV ∗
+               (l2 +ₗ i) ↦ᵣ∗ replicate (Z.to_nat (sz-i)) NONEV ∗
+               i1 ↦ₗ #i ∗ i2 ↦ᵣ #i)%I.
+
+
+  Lemma new_allocator_spec (sz : Z) ξ Φ :
+    0 < sz →
+    (∀ (a1 a2 : val),
+        (∀ (α : slevel), ⟦ tarrow (tint α) (toption (tref (tint α))) Low ⟧ ξ a1 a2) -∗
+        Φ a1 a2) -∗
+    DWP new_allocator #sz & new_allocator #sz : Φ.
+  Proof.
+    iIntros (Hsz) "H".
+    dwp_rec. dwp_pures.
+    dwp_bind (AllocN _ _) (AllocN _ _).
+    (* allocN spec *)
+    set (meta_token1 := @meta_token _ _ _ _ _ heapDG_gen_heapG1).
+    set (meta_token2 := @meta_token _ _ _ _ _ heapDG_gen_heapG2).
+    pose (Ψ1 := (λ v, ∃ l : loc, ⌜v = #l⌝ ∗ l ↦ₗ∗ replicate (Z.to_nat sz) NONEV ∗
+                 ([∗ list] i ∈ seq 0 (Z.to_nat sz), meta_token1 (l +ₗ Z.of_nat i) ⊤))%I).
+    pose (Ψ2 := (λ v, ∃ l : loc, ⌜v = #l⌝ ∗ l ↦ᵣ∗ replicate (Z.to_nat sz) NONEV ∗
+                 ([∗ list] i ∈ seq 0 (Z.to_nat sz), meta_token2 (l +ₗ Z.of_nat i) ⊤))%I).
+    iApply (dwp_atomic_lift_wp Ψ1 Ψ2).
+    - iApply twp_allocN; try done.
+      iIntros (l) "[Hl Hmeta]". iExists l.
+      iSplit; eauto. iSplitL "Hl". iExact "Hl". iFrame.
+    - iApply twp_allocN; try done.
+      iIntros (l) "[Hl Hmeta]". iExists l.
+      iSplit; eauto. iSplitL "Hl". iExact "Hl". iFrame.
+    - iIntros (? ?). iDestruct 1 as (l1) "[-> [Hl1 Hmeta1]]".
+      iDestruct 1 as (l2) "[-> [Hl2 Hmeta2]]".
+      (* / allocN spec *)
+      iClear "Hmeta1 Hmeta2".
+
+      iNext. dwp_pures.
+      dwp_bind (ref _)%E (ref _)%E.
+      iApply dwp_alloc. iIntros (i1 i2) "Hi1 Hi2". iNext. dwp_pures.
+
+      dwp_bind (newlock #()) (newlock #()).
+      iApply (newlock_spec aN (allocator_inv l1 l2 i1 i2 sz) with "[Hl1 Hl2 Hi1 Hi2]").
+      { iExists 0. rewrite !loc_add_0. assert (sz - 0 = sz) as -> by lia.
+        iFrame. iPureIntro. lia. }
+      iIntros (γ lk1 lk2) "#Hlk". dwp_pures.
+
+      iApply dwp_value. iModIntro. iApply "H". iIntros (α).
+      rewrite interp_eq. iModIntro. iIntros (v1 v2) "#Hv".
+      dwp_pures.
+
+      dwp_bind (acquire _)%E (acquire _)%E.
+      iApply (acquire_spec with "Hlk"). iIntros "Hlocked".
+      iDestruct 1 as (i Hi) "(Hl1&Hl2&Hi1&Hi2)".
+
+      dwp_pures. dwp_rec. dwp_pures.
+      dwp_bind (! _)%E (! _)%E. iApply (dwp_load with "Hi1 Hi2").
+      iIntros "Hi1 Hi2". iNext. dwp_pures.
+      case_bool_decide; dwp_pures.
+      + dwp_bind (release _)%E (release _)%E.
+        iApply (release_spec with "Hlk Hlocked [Hl1 Hl2 Hi1 Hi2]").
+        { iExists i. iSplit. done. iFrame. }
+        dwp_pures. iApply logrel_none.
+      + dwp_bind (_ <- _)%E (_ <- _)%E.
+        iApply (dwp_store with "Hi1 Hi2"). iIntros "Hi1 Hi2".
+        iNext. dwp_pures.
+        assert (Z.to_nat (sz - i) = S (Z.to_nat (sz - (i + 1)))) as ->.
+        { destruct Hi. rewrite -Z2Nat.inj_succ; last by lia.
+          f_equal. lia. }
+        simpl. rewrite array1_cons array2_cons.
+        iDestruct "Hl1" as "[Hcell1 Hl1]".
+        iDestruct "Hl2" as "[Hcell2 Hl2]".
+        dwp_bind (_ <- _)%E (_ <- _)%E.
+        iApply (dwp_store with "Hcell1 Hcell2").
+        iIntros "Hcell1 Hcell2". iNext. dwp_pures.
+
+        dwp_bind (release _) (release _).
+        iApply (release_spec with "Hlk Hlocked [Hl1 Hl2 Hi1 Hi2]").
+        { iExists (i+1). iSplit.
+          - iPureIntro; lia.
+          - iFrame. rewrite !loc_add_assoc. iFrame. }
+        dwp_pures. iApply logrel_some.
+        iMod (interp_ref_alloc with "Hcell1 Hcell2 Hv") as "#Hcell".
+        iApply dwp_value. eauto.
+  Qed.
+
+End proof.
